Rework memory layout
I now think it is roughly following the layout used on x86

examples/ag32/compilation/proofs/hello_ag32ProofScript.sml
@@ -26,6 +26,22 @@ val LENGTH_data =
 val memory_size_def = Define`
   memory_size = 128 * 2 ** 20`;
 
+val heap_size_def = Define`
+  heap_size = 120 * 2 ** 20`;
+
+(*
+  hz = heap_size is the heap+stack size in mebibytes
+  r0 gives the lowest software-usable address
+  r0 .. r0 + 64 is used by the FFI implementation
+  r0 + 64 .. r0 + hzMiB is the CakeML heap+stack space
+  r0 + hzMiB .. r0 + hzMiB + 4 * LENGTH data is the bitmaps
+  r0 + hzMiB + 4 * LENGTH data is the FFI PC
+  r0 + hzMiB + 4 * LENGTH data + 16 is the ccache PC
+  r0 + hzMiB + 4 * LENGTH data + 32 is the halt PC
+  r0 + hzMiB + 4 * LENGTH data + 48 is the initial PC
+  r0 + hzMiB + 4 * LENGTH data + 48 .. r0 + hzMiB + 4 * LENGTH data + 48 + LENGTH code is the code
+*)
+
 val hello_machine_config_def = Define`
   hello_machine_config r0 = <|
     target := ag32_target;
@@ -35,10 +51,12 @@ val hello_machine_config_def = Define`
     len2_reg := 4;
     callee_saved_regs := [60; 61; 62];
     ffi_names := ^(rand(rconc ffi_names));
-    ffi_entry_pcs := [r0 + 64w];
-    ccache_pc := r0 + 64w +  n2w ffi_offset;
-    halt_pc := r0 + 64w + n2w (2 * ffi_offset) ;
-    prog_addresses := { w | r0 + 64w + n2w (3 * ffi_offset) <=+ w ∧ w <+ r0 + (n2w memory_size) };
+    ffi_entry_pcs := [r0 + n2w (heap_size + 4 * LENGTH data + 0 * ffi_offset)];
+    ccache_pc      := r0 + n2w (heap_size + 4 * LENGTH data + 1 * ffi_offset);
+    halt_pc        := r0 + n2w (heap_size + 4 * LENGTH data + 2 * ffi_offset);
+    prog_addresses :=
+      { w | r0 + 64w <=+ w ∧ w <+ r0 + n2w (heap_size + 4 * LENGTH data) } ∪
+      { w | r0 + n2w (heap_size + 4 * LENGTH data + 3 * ffi_offset) <=+ w ∧ w <+ r0 + (n2w memory_size) };
     next_interfer := K I ;
     ccache_interfer := K (λ(_,_,ms). ms with PC := (ms.R 0w))
   |>`
@@ -48,24 +66,34 @@ val is_ag32_machine_config_hello_machine_config = Q.store_thm("is_ag32_machine_c
 
 val hello_init_memory_def = Define`
   hello_init_memory r0 (k:word32) =
-     if r0 + 112w <=+ k ∧ k <+ r0 + 112w + n2w (LENGTH code) then
-       EL (w2n (k - (r0 + 112w))) code
-     else if r0 + 112w + n2w (LENGTH code) <=+ k ∧ k <+ r0 + 112w + n2w (LENGTH code) + n2w (4 * LENGTH data) then
-       get_byte (k - (r0 + 112w + n2w (LENGTH code)))
-         (EL (w2n (k - (r0 + 112w + n2w (LENGTH code)))) data) F
+     if r0 + n2w heap_size <=+ k ∧ k <+ r0 + n2w (heap_size + 4 * LENGTH data) then
+       get_byte k (EL (w2n (k - (r0 + n2w heap_size))) data) F
+     else if r0 + n2w (heap_size + 4 * LENGTH data + 3 * ffi_offset) <=+ k ∧
+             k <+ r0 + n2w (heap_size + 4 * LENGTH data + 3 * ffi_offset + LENGTH code) then
+       EL (w2n (k - (r0 + n2w (heap_size + 4 * LENGTH data + 3 * ffi_offset)))) code
+     else if r0 + 64w + 0w * bytes_in_word ≤ k ∧ k < r0 + 64w + 1w * bytes_in_word then
+       get_byte k (r0 + n2w heap_size) F
+     else if r0 + 64w + 1w * bytes_in_word ≤ k ∧ k < r0 + 64w + 2w * bytes_in_word then
+       get_byte k (r0 + n2w heap_size + bytes_in_word * n2w (LENGTH data)) F
+     else if r0 + 64w + 2w * bytes_in_word ≤ k ∧ k < r0 + 64w + 3w * bytes_in_word then
+       get_byte k (r0 + n2w heap_size + bytes_in_word * n2w (LENGTH data)) F
+     else if r0 + 64w + 3w * bytes_in_word ≤ k ∧ k < r0 + 64w + 4w * bytes_in_word then
+       get_byte k (r0 + n2w (heap_size + 4 * LENGTH data + 3 * ffi_offset + LENGTH code)) F
+     else if r0 + 64w + 4w * bytes_in_word ≤ k ∧ k < r0 + 64w + 5w * bytes_in_word then
+       get_byte k (r0 + n2w (heap_size + 4 * LENGTH data + 3 * ffi_offset + LENGTH code)) F
      else (0w:word8)`;
 
 val hello_init_regs_def = Define`
   hello_init_regs r0 (k:num) =
   if k = 2 then
-    r0 + 112w + n2w (LENGTH code)
+    r0 + 64w
   else if k = 4 then
-    r0 + n2w memory_size
+    r0 + n2w heap_size
   else (0w:word32)`;
 
 val hello_init_ag32_state_def = Define`
   hello_init_ag32_state (r0:word32) = <|
-    PC := r0 + 64w + n2w (3 * ffi_offset) ;
+    PC := r0 + n2w (heap_size + 4 * LENGTH data + 3 * ffi_offset);
     MEM := hello_init_memory r0;
     R := hello_init_regs r0 o w2n
   |>`;
@@ -76,21 +104,21 @@ val hello_init_asm_state_def = Define`
     lr := 0 ;
     failed := F ;
     align := 2 ;
-    pc := r0 + 64w + n2w (3 * ffi_offset);
-    mem := hello_init_memory r0;
+    pc := (hello_init_ag32_state r0).PC;
+    mem := (hello_init_ag32_state r0).MEM;
     mem_domain := (hello_machine_config r0).prog_addresses ;
     regs := hello_init_regs r0
   |>`;
 
 val hello_good_init_state = Q.store_thm("hello_good_init_state",
-  `aligned 2 r0 ∧ w2n r0 + 64 + 3 * ffi_offset + memory_size < dimword(:32) ⇒
+  `aligned 2 r0 ∧ w2n r0 + memory_size < dimword(:32) ⇒
    good_init_state (hello_machine_config r0) (hello_init_ag32_state r0)
      ag_ffi code 0 (hello_init_asm_state r0)
      (λk. Word (bytes_to_word 4 0w (GENLIST (λn. hello_init_memory r0 (k + n2w n)) 4) 0w F))
        ({w | (hello_init_asm_state r0).regs 2 <=+ w ∧
              w <+ (hello_init_asm_state r0).regs 4}
-        ∪ {w | r0 + 64w + n2w(3 * ffi_offset + LENGTH code) <=+ w ∧
-               w <+ r0 + 64w + n2w(3 * ffi_offset + LENGTH code + 4 * LENGTH data) })
+        ∪ {w | r0 + n2w heap_size <=+ w ∧
+               w <+ r0 + n2w(heap_size + 4 * LENGTH data) })
      io_regs (K(K NONE))`,
   strip_tac
   \\ simp[lab_to_targetProofTheory.good_init_state_def]
@@ -104,12 +132,8 @@ val hello_good_init_state = Q.store_thm("hello_good_init_state",
       \\ (alignmentTheory.aligned_add_sub_cor
           |> SPEC_ALL |> UNDISCH |> CONJUNCT1 |> DISCH_ALL
           |> irule)
-      \\ reverse conj_tac >- EVAL_TAC
-      \\ (alignmentTheory.aligned_add_sub_cor
-          |> SPEC_ALL |> UNDISCH |> CONJUNCT1 |> DISCH_ALL
-          |> irule)
-      \\ reverse conj_tac >- EVAL_TAC
-      \\ fs[] )
+      \\ simp[LENGTH_data]
+      \\ EVAL_TAC)
     \\ conj_tac >- EVAL_TAC
     \\ conj_tac >- (EVAL_TAC \\ rw[])
     \\ EVAL_TAC \\ rw[] )
@@ -126,7 +150,7 @@ val hello_good_init_state = Q.store_thm("hello_good_init_state",
     \\ qx_gen_tac`m`
     \\ cheat (* target_configured needs to be fixed *) )
   \\ conj_tac >- EVAL_TAC
-  \\ `r0 + 64w + 48w && 3w = 0w` by (
+  \\ `r0 + n2w (heap_size + 4 * LENGTH data + 3 * ffi_offset) && 3w = 0w` by (
     fs[alignmentTheory.aligned_bitwise_and]
     \\ Cases_on`r0`
     \\ simp[word_add_n2w]
@@ -135,8 +159,9 @@ val hello_good_init_state = Q.store_thm("hello_good_init_state",
     \\ qpat_x_assum`_ = 0w`mp_tac
     \\ once_rewrite_tac[WORD_AND_COMM]
     \\ rewrite_tac[addressTheory.n2w_and_3]
+    \\ EVAL_TAC
     \\ simp[] )
-  \\ `r0 + 64w + 48w && 1w = 0w` by (
+  \\ `r0 + n2w (heap_size + 4 * LENGTH data + 3 * ffi_offset) && 1w = 0w` by (
     fs[alignmentTheory.aligned_bitwise_and]
     \\ Cases_on`r0`
     \\ simp[word_add_n2w]
@@ -145,7 +170,8 @@ val hello_good_init_state = Q.store_thm("hello_good_init_state",
     \\ qpat_x_assum`_ && n2w n = 0w`mp_tac
     \\ once_rewrite_tac[WORD_AND_COMM]
     \\ rewrite_tac[addressTheory.n2w_and_3]
-    \\ simp[]
+    \\ EVAL_TAC
+    \\ simp[LENGTH_data]
     \\ DEP_ONCE_REWRITE_TAC[LESS_MOD]
     \\ conj_tac
     >- (
@@ -168,15 +194,17 @@ val hello_good_init_state = Q.store_thm("hello_good_init_state",
       qpat_x_assum`_ < _`mp_tac
       \\ EVAL_TAC
       \\ Cases_on`r0`
-      \\ simp[WORD_LOWER_OR_EQ,WORD_NOT_LOWER,word_add_n2w,word_ls_n2w] )
+      \\ simp[WORD_LOWER_OR_EQ,WORD_NOT_LOWER,word_add_n2w,word_ls_n2w,LENGTH_data] )
     \\ conj_tac >- (
       qpat_x_assum`_ < _`mp_tac
       \\ EVAL_TAC
       \\ Cases_on`r0`
-      \\ simp[WORD_LOWER_OR_EQ,WORD_NOT_LOWER,word_add_n2w,word_ls_n2w] )
-    \\ conj_tac >- (EVAL_TAC \\ simp[])
-    \\ conj_tac >- (EVAL_TAC \\ simp[])
-    \\ conj_tac >- ( EVAL_TAC \\ fs[] )
+      \\ simp[WORD_LOWER_OR_EQ,WORD_NOT_LOWER,word_add_n2w,word_ls_n2w,LENGTH_data] )
+    \\ conj_tac >- (EVAL_TAC \\ simp[LENGTH_data])
+    \\ conj_tac >- (EVAL_TAC \\ simp[LENGTH_data])
+    \\ conj_tac >- (
+      qpat_x_assum`_ && 1w = _` mp_tac
+      \\ EVAL_TAC \\ fs[] )
     \\ rewrite_tac[EVAL``(hello_machine_config r0).ffi_names``]
     \\ reverse Cases >- rw[]
     \\ strip_tac
@@ -184,19 +212,21 @@ val hello_good_init_state = Q.store_thm("hello_good_init_state",
       qpat_x_assum`_ < dimword _`mp_tac
       \\ EVAL_TAC
       \\ Cases_on`r0`
-      \\ simp[WORD_LOWER_OR_EQ,WORD_NOT_LOWER,word_add_n2w,word_ls_n2w] )
+      \\ simp[WORD_LOWER_OR_EQ,WORD_NOT_LOWER,word_add_n2w,word_ls_n2w,LENGTH_data] )
     \\ conj_tac >- (
       qpat_x_assum`_ < dimword _`mp_tac
       \\ EVAL_TAC
       \\ Cases_on`r0`
-      \\ simp[WORD_LOWER_OR_EQ,WORD_NOT_LOWER,word_add_n2w,word_ls_n2w] )
+      \\ simp[WORD_LOWER_OR_EQ,WORD_NOT_LOWER,word_add_n2w,word_ls_n2w,LENGTH_data] )
     \\ conj_tac >- (
       qpat_x_assum`_ < dimword _`mp_tac
       \\ EVAL_TAC
       \\ Cases_on`r0`
-      \\ simp[WORD_LOWER_OR_EQ,WORD_NOT_LOWER,word_add_n2w,word_ls_n2w] )
-    \\ EVAL_TAC \\ rw[] )
-  \\ conj_tac >- ( EVAL_TAC \\ fs[] )
+      \\ simp[WORD_LOWER_OR_EQ,WORD_NOT_LOWER,word_add_n2w,word_ls_n2w,LENGTH_data] )
+    \\ EVAL_TAC \\ rw[LENGTH_data] )
+  \\ conj_tac >- (
+    qpat_x_assum`_ && 3w = _`mp_tac
+    \\ EVAL_TAC \\ fs[LENGTH_data] )
   \\ conj_tac >- (
     rw[asmPropsTheory.interference_ok_def]
     \\ simp[EVAL``(hello_machine_config r0).target``]
@@ -213,7 +243,7 @@ val hello_good_init_state = Q.store_thm("hello_good_init_state",
     \\ qpat_x_assum`_ < dimword _`mp_tac
     \\ EVAL_TAC
     \\ Cases_on`r0`
-    \\ fs[word_add_n2w, word_ls_n2w, word_lo_n2w, LENGTH_code]
+    \\ fs[word_add_n2w, word_ls_n2w, word_lo_n2w, LENGTH_code, LENGTH_data]
     \\ simp[GSYM word_add_n2w, WORD_LEFT_ADD_DISTRIB])
   \\ conj_tac >- cheat (* can this be proved from the previous conjunct? *)
   \\ conj_tac >- (
@@ -233,10 +263,11 @@ val hello_good_init_state = Q.store_thm("hello_good_init_state",
     \\ strip_tac
     \\ Cases
     \\ fs[word_ls_n2w, word_lo_n2w, word_slice_n2w]
-    \\ cheat (* annoying word proofs: bitmap_dm is word addressable *)
-  )
+    \\ cheat (* annoying word proofs: bitmap_dm is word addressable *))
   \\ conj_tac >- (
-    rw[hello_init_asm_state_def, EVAL``(hello_machine_config r0).target.config``]
+    rw[hello_init_asm_state_def,
+       EVAL``(hello_machine_config r0).target.config``,
+       EVAL``(hello_init_ag32_state r0).MEM``]
     \\ `∃i. (a = i + byte_align a) ∧ w2n i < 4`
     by (
       rw[alignmentTheory.byte_align_def]
@@ -304,8 +335,13 @@ val lemma = prove(
     \\ strip_tac
     \\ Cases
     \\ Cases_on`r0`
-    \\ fs[word_add_n2w,word_ls_n2w,word_lo_n2w]
-    \\ CCONTR_TAC \\ fs[] \\ fs[] \\ rw[]
+    \\ fs[word_add_n2w,word_ls_n2w,word_lo_n2w] )
+  \\ conj_tac
+  >- (
+    rw[EVAL``(hello_init_asm_state r0).regs``, LENGTH_data]
+    \\ rw[hello_init_regs_def]
+    \\ cheat (* prove some memory lookup rewrites separately *) )
+  \\ conj_tac
 *)
 
 val _ = export_theory();
